WIP: imp2csm compiler ver.2.0

imp/Imp.v
@@ -21,7 +21,7 @@ Definition var : Set := string.
 (** Expressions are made of variables, constant literals, and arithmetic operations. *)
 Inductive expr : Type :=
 | Var (_ : var)
-| Lit (_ : val)
+| Lit (_ : Z)
 | Plus  (_ _ : expr)
 | Minus (_ _ : expr)
 | Mult  (_ _ : expr)
@@ -51,191 +51,8 @@ Record function : Type := mk_function {
   fn_body : stmt
 }.
 
-(* ========================================================================== *)
-(** ** Semantics *)
 
-(** Get/Set function local variables *)
-Variant ImpState : Type -> Type :=
-| GetVar (x : var) : ImpState val
-| SetVar (x : var) (v : val) : ImpState unit.
 
-(** Get pointer to a global variable/function *)
-Variant GlobEnv : Type -> Type :=
-| GetPtr (x: gname) : GlobEnv val
-| GetName (p: val) : GlobEnv gname.
-
-Section Denote.
-
-  Context `{Σ: GRA.t}.
-  Context {eff : Type -> Type}.
-  Context {HasGlobVar: GlobEnv -< eff}.
-  Context {HasImpState : ImpState -< eff}.
-  Context {HasCall : callE -< eff}.
-  Context {HasEvent : eventE -< eff}.
-
-  (** Denotation of expressions *)
-  Fixpoint denote_expr (e : expr) : itree eff val :=
-    match e with
-    | Var v     => u <- trigger (GetVar v) ;; assume (wf_val u) ;;; Ret u
-    | Lit n     => assume (wf_val n) ;;; Ret n
-    | Plus a b  => l <- denote_expr a ;; r <- denote_expr b ;; u <- (vadd l r)? ;; assume (wf_val u) ;;; Ret u
-    | Minus a b => l <- denote_expr a ;; r <- denote_expr b ;; u <- (vsub l r)? ;; assume (wf_val u) ;;; Ret u
-    | Mult a b  => l <- denote_expr a ;; r <- denote_expr b ;; u <- (vmul l r)? ;; assume (wf_val u) ;;; Ret u
-    end.
-
-  (** Denotation of statements *)
-  Definition is_true (v : val) : option bool :=
-    match v with
-    | Vint n => if (n =? 0)%Z then Some false else Some true
-    | _ => None
-    end.
-
-  Fixpoint denote_exprs_acc (es : list expr) (acc : list val) : itree eff (list val) :=
-    match es with
-    | [] => Ret acc
-    | e :: s =>
-      v <- denote_expr e;; denote_exprs_acc s (acc ++ [v])
-    end.
-
-  Fixpoint denote_exprs (es : list expr) : itree eff (list val) :=
-    match es with
-    | [] => Ret []
-    | e :: s =>
-      v <- denote_expr e;;
-      vs <- denote_exprs s;;
-      Ret (v :: vs)
-    end.
-
-  Definition call_mem f :=
-    rel_dec f "alloc" || rel_dec f "free" || rel_dec f "load" || rel_dec f "store" || rel_dec f "cmp" || rel_dec f "main".
-
-  Fixpoint denote_stmt (s : stmt) : itree eff val :=
-    match s with
-    | Skip => tau;; Ret Vundef
-    | Assign x e =>
-      v <- denote_expr e;; trigger (SetVar x v);;; tau;; Ret Vundef
-    | Seq a b =>
-      tau;; denote_stmt a;;; denote_stmt b
-    | If i t e =>
-      v <- denote_expr i;; `b: bool <- (is_true v)?;; tau;;
-      if b then (denote_stmt t) else (denote_stmt e)
-
-    | CallFun x f args =>
-      if (call_mem f)
-      then triggerUB
-      else
-        eval_args <- denote_exprs args;;
-        v <- trigger (Call f (eval_args↑));; v <- unwrapN (v↓);;
-        trigger (SetVar x v);;; tau;; Ret Vundef
-
-    | CallPtr x e args =>
-      p <- denote_expr e;; f <- trigger (GetName p);;
-      if (call_mem f)
-      then triggerUB
-      else
-        eval_args <- denote_exprs args;;
-        v <- trigger (Call f (eval_args↑));; v <- unwrapN (v↓);;
-        trigger (SetVar x v);;; tau;; Ret Vundef
-
-    | CallSys x f args =>
-      eval_args <- denote_exprs args;;
-      v <- trigger (Syscall f eval_args top1);;
-      trigger (SetVar x v);;; tau;; Ret Vundef
-
-    | AddrOf x X =>
-      v <- trigger (GetPtr X);; trigger (SetVar x v);;; tau;; Ret Vundef
-    | Malloc x se =>
-      s <- denote_expr se;;
-      v <- trigger (Call "alloc" ([s]↑));; v <- unwrapN(v↓);;
-      trigger (SetVar x v);;; tau;; Ret Vundef
-    | Free pe =>
-      p <- denote_expr pe;;
-      trigger (Call "free" ([p]↑));;; tau;; Ret Vundef
-    | Load x pe =>
-      p <- denote_expr pe;;
-      v <- trigger (Call "load" ([p]↑));; v <- unwrapN(v↓);;
-      trigger (SetVar x v);;; tau;; Ret Vundef
-    | Store pe ve =>
-      p <- denote_expr pe;; v <- denote_expr ve;;
-      trigger (Call "store" ([p ; v]↑));;; tau;; Ret Vundef
-    | Cmp x ae be =>
-      a <- denote_expr ae;; b <- denote_expr be;;
-      v <- trigger (Call "cmp" ([a ; b]↑));; v <- unwrapN (v↓);;
-      trigger (SetVar x v);;; tau;; Ret Vundef
-
-    end.
-
-End Denote.
-
-(* ========================================================================== *)
-(** ** Interpretation *)
-
-Section Interp.
-
-  Context `{Σ: GRA.t}.
-  Definition effs := GlobEnv +' ImpState +' Es.
-
-  Definition handle_GlobEnv {eff} `{eventE -< eff} (ge: SkEnv.t) : GlobEnv ~> (itree eff) :=
-    fun _ e =>
-      match e with
-      | GetPtr X =>
-        r <- (ge.(SkEnv.id2blk) X)?;; Ret (Vptr r 0)
-      | GetName p =>
-        match p with
-        | Vptr n 0 => x <- (ge.(SkEnv.blk2id) n)?;; Ret (x)
-        | _ => triggerUB
-        end
-      end.
-
-  Definition interp_GlobEnv {eff} `{eventE -< eff} (ge: SkEnv.t) : itree (GlobEnv +' eff) ~> (itree eff) :=
-    interp (case_ (handle_GlobEnv ge) ((fun T e => trigger e) : eff ~> itree eff)).
-
-  (** function local environment *)
-  Definition lenv := alist var val.
-  Definition handle_ImpState {eff} `{eventE -< eff} : ImpState ~> stateT lenv (itree eff) :=
-    fun _ e le =>
-      match e with
-      | GetVar x => r <- unwrapU (alist_find x le);; Ret (le, r)
-      | SetVar x v => Ret (alist_add x v le, tt)
-      end.
-
-  Definition interp_ImpState {eff} `{eventE -< eff}: itree (ImpState +' eff) ~> stateT lenv (itree eff) :=
-    State.interp_state (case_ handle_ImpState ModSem.pure_state).
-
-  (* Definition interp_imp ge le (itr : itree effs val) := *)
-  (*   interp_ImpState (interp_GlobEnv ge itr) le. *)
-
-  Definition interp_imp ge : itree effs ~> stateT lenv (itree Es) :=
-    fun _ itr le => interp_ImpState (interp_GlobEnv ge itr) le.
-
-  (* 'return' is a fixed register, holding the return value of this function. *)
-  Fixpoint init_lenv xs : lenv :=
-    match xs with
-    | [] => [("return", Vundef); ("_", Vundef)]
-    | x :: t => (x, Vundef) :: (init_lenv t)
-    end
-  .
-
-  Fixpoint init_args params args (acc: lenv) : option lenv :=
-    match params, args with
-    | [], [] => Some acc
-    | x :: part, v :: argt =>
-      init_args part argt (alist_add x v acc)
-    | _, _ => None
-    end
-  .
-
-  Definition eval_imp (ge: SkEnv.t) (f: function) (args: list val) : itree Es val :=
-    match (init_args f.(fn_params) args []) with
-    | Some iargs =>
-      '(_, retv) <- (interp_imp ge (tau;; denote_stmt f.(fn_body) ;;; retv <- (denote_expr (Var "return")) ;; Ret retv) ((init_lenv f.(fn_vars))++iargs));; Ret retv
-    | None => triggerUB
-    end
-  .
-
-End Interp.
-
-(* ========================================================================== *)
 (** ** Program *)
 
 (** program components *)
@@ -285,8 +102,220 @@ Definition lift (p : program) : programL :=
     p.(public) p.(defs).
 
 Coercion lift : program >-> programL.
-(* Global Opaque imp_lift. *)
 
+
+
+
+
+(* ========================================================================== *)
+(** ** Semantics *)
+
+(** Get/Set function local variables *)
+Variant ImpState : Type -> Type :=
+| GetVar (x : var) : ImpState val
+| SetVar (x : var) (v : val) : ImpState unit.
+
+(** Get pointer to a global variable/function *)
+Variant GlobEnv : Type -> Type :=
+| GetPtr (x: gname) : GlobEnv val
+| GetName (p: val) : GlobEnv gname.
+
+Section Denote.
+
+  Context `{Σ: GRA.t}.
+  Context {eff : Type -> Type}.
+  Context {HasGlobVar: GlobEnv -< eff}.
+  Context {HasImpState : ImpState -< eff}.
+  Context {HasCall : callE -< eff}.
+  Context {HasEvent : eventE -< eff}.
+
+  (** Denotation of expressions *)
+  Fixpoint denote_expr (e : expr) : itree eff val :=
+    match e with
+    | Var v     => u <- trigger (GetVar v) ;; assume (wf_val u) ;;; Ret u
+    | Lit n     => assume (wf_val (Vint n)) ;;; Ret (Vint n)
+    | Plus a b  => l <- denote_expr a ;; r <- denote_expr b ;; u <- (vadd l r)? ;; assume (wf_val u) ;;; Ret u
+    | Minus a b => l <- denote_expr a ;; r <- denote_expr b ;; u <- (vsub l r)? ;; assume (wf_val u) ;;; Ret u
+    | Mult a b  => l <- denote_expr a ;; r <- denote_expr b ;; u <- (vmul l r)? ;; assume (wf_val u) ;;; Ret u
+    end.
+
+  (** Denotation of statements *)
+  Definition is_true (v : val) : option bool :=
+    match v with
+    | Vint n => if (n =? 0)%Z then Some false else Some true
+    | _ => None
+    end.
+
+  Fixpoint denote_exprs_acc (es : list expr) (acc : list val) : itree eff (list val) :=
+    match es with
+    | [] => Ret acc
+    | e :: s =>
+      v <- denote_expr e;; denote_exprs_acc s (acc ++ [v])
+    end.
+
+  Fixpoint denote_exprs (es : list expr) : itree eff (list val) :=
+    match es with
+    | [] => Ret []
+    | e :: s =>
+      v <- denote_expr e;;
+      vs <- denote_exprs s;;
+      Ret (v :: vs)
+    end.
+
+  Definition call_ban f :=
+    rel_dec f "alloc" || rel_dec f "free" || rel_dec f "load" || rel_dec f "store" || rel_dec f "cmp" || rel_dec f "main".
+
+  Fixpoint denote_stmt (efs : extFuns) (s : stmt) : itree eff val :=
+    match s with
+    | Skip => tau;; Ret Vundef
+    | Assign x e =>
+      v <- denote_expr e;; trigger (SetVar x v);;; tau;; Ret Vundef
+    | Seq a b =>
+      tau;; denote_stmt efs a;;; denote_stmt efs b
+    | If i t e =>
+      v <- denote_expr i;; `b: bool <- (is_true v)?;; tau;;
+      if b then (denote_stmt efs t) else (denote_stmt efs e)
+
+    | CallFun x f args =>
+      if (call_ban f)
+      then triggerUB
+      else
+        eval_args <- denote_exprs args;;
+        v <- trigger (Call f (eval_args↑));; v <- unwrapN (v↓);;
+        trigger (SetVar x v);;; tau;; Ret Vundef
+
+    | CallPtr x e args =>
+      assume (match e with | Var _ => True | _ => False end);;;
+      p <- denote_expr e;; f <- trigger (GetName p);;
+      if (call_ban f)
+      then triggerUB
+      else
+        eval_args <- denote_exprs args;;
+        v <- trigger (Call f (eval_args↑));; v <- unwrapN (v↓);;
+        trigger (SetVar x v);;; tau;; Ret Vundef
+
+    | CallSys x f args =>
+      sig <- (alist_find f efs)? ;; assume (sig = List.length args);;;
+      eval_args <- denote_exprs args;;
+      v <- trigger (Syscall f eval_args top1);;
+      trigger (SetVar x v);;; tau;; Ret Vundef
+
+    | AddrOf x X =>
+      v <- trigger (GetPtr X);; trigger (SetVar x v);;; tau;; Ret Vundef
+    | Malloc x se =>
+      s <- denote_expr se;;
+      v <- trigger (Call "alloc" ([s]↑));; v <- unwrapN(v↓);;
+      trigger (SetVar x v);;; tau;; Ret Vundef
+    | Free pe =>
+      p <- denote_expr pe;;
+      trigger (Call "free" ([p]↑));;; tau;; Ret Vundef
+    | Load x pe =>
+      p <- denote_expr pe;;
+      v <- trigger (Call "load" ([p]↑));; v <- unwrapN(v↓);;
+      trigger (SetVar x v);;; tau;; Ret Vundef
+    | Store pe ve =>
+      p <- denote_expr pe;; v <- denote_expr ve;;
+      trigger (Call "store" ([p ; v]↑));;; tau;; Ret Vundef
+    | Cmp x ae be =>
+      a <- denote_expr ae;; b <- denote_expr be;;
+      v <- trigger (Call "cmp" ([a ; b]↑));; v <- unwrapN (v↓);;
+      trigger (SetVar x v);;; tau;; Ret Vundef
+
+    end.
+
+End Denote.
+
+
+
+
+
+(* ========================================================================== *)
+(** ** Interpretation *)
+
+Section Interp.
+
+  Context `{Σ: GRA.t}.
+  Definition effs := GlobEnv +' ImpState +' Es.
+
+  Definition handle_GlobEnv {eff} `{eventE -< eff} (ge: SkEnv.t) : GlobEnv ~> (itree eff) :=
+    fun _ e =>
+      match e with
+      | GetPtr X =>
+        r <- (ge.(SkEnv.id2blk) X)?;; Ret (Vptr r 0)
+      | GetName p =>
+        match p with
+        | Vptr n 0 => x <- (ge.(SkEnv.blk2id) n)?;; Ret (x)
+        | _ => triggerUB
+        end
+      end.
+
+  Definition interp_GlobEnv {eff} `{eventE -< eff} (ge: SkEnv.t) : itree (GlobEnv +' eff) ~> (itree eff) :=
+    interp (case_ (handle_GlobEnv ge) ((fun T e => trigger e) : eff ~> itree eff)).
+
+  (** function local environment *)
+  Definition lenv := alist var val.
+  Definition handle_ImpState {eff} `{eventE -< eff} : ImpState ~> stateT lenv (itree eff) :=
+    fun _ e le =>
+      match e with
+      | GetVar x => r <- unwrapU (alist_find x le);; Ret (le, r)
+      | SetVar x v => Ret (alist_add x v le, tt)
+      end.
+
+  Definition interp_ImpState {eff} `{eventE -< eff}: itree (ImpState +' eff) ~> stateT lenv (itree eff) :=
+    State.interp_state (case_ handle_ImpState ModSem.pure_state).
+
+  (* Definition interp_imp ge le (itr : itree effs val) := *)
+  (*   interp_ImpState (interp_GlobEnv ge itr) le. *)
+
+  Definition interp_imp ge : itree effs ~> stateT lenv (itree Es) :=
+    fun _ itr le => interp_ImpState (interp_GlobEnv ge itr) le.
+
+  Fixpoint init_lenv xs : lenv :=
+    match xs with
+    | [] => []
+    | x :: t => (x, Vundef) :: (init_lenv t)
+    end
+  .
+
+  Fixpoint init_args params args (acc: lenv) : option lenv :=
+    match params, args with
+    | [], [] => Some acc
+    | x :: part, v :: argt =>
+      init_args part argt (alist_add x v acc)
+    | _, _ => None
+    end
+  .
+
+  Lemma init_args_prop :
+    forall params args acc le
+      (INITSOME: init_args params args acc = Some le),
+      <<INITLEN: List.length params = List.length args>>.
+  Proof.
+    induction params; i; ss; clarify.
+    { destruct args; ss; clarify. }
+    destruct args; ss; clarify. apply IHparams in INITSOME. red. rewrite INITSOME. ss.
+  Qed.
+
+  (* 'return' is a fixed register, holding the return value of this function. *)
+  (* '_' is a black hole register, holding garbage *)
+  Definition eval_imp (ge: SkEnv.t) (efs: extFuns) (f: function) (args: list val) : itree Es val :=
+    let vars := f.(fn_vars) ++ ["return"; "_"] in
+    let params := f.(fn_params) in
+    assume (NoDup (params ++ vars));;;
+    match (init_args params args []) with
+    | Some iargs =>
+      '(_, retv) <- (interp_imp ge (tau;; (denote_stmt efs f.(fn_body));;; retv <- (denote_expr (Var "return")) ;; Ret retv)
+                                    ((init_lenv vars) ++ iargs));; Ret retv
+    | None => triggerUB
+    end.
+
+End Interp.
+
+
+
+
+
+(* ========================================================================== *)
 (**** ModSem ****)
 Module ImpMod.
 Section MODSEM.
@@ -297,7 +326,7 @@ Section MODSEM.
   (* Instance Initial_void1 : @Initial (Type -> Type) IFun void1 := @elim_void1. (*** TODO: move to ITreelib ***) *)
 
   Definition modsem (m : program) (ge: SkEnv.t) : ModSem.t := {|
-    ModSem.fnsems := List.map (fun '(fn, f) => (fn, cfun (eval_imp ge f))) m.(prog_funs);
+    ModSem.fnsems := List.map (fun '(fn, f) => (fn, cfun (eval_imp ge m.(ext_funs) f))) m.(prog_funs);
     ModSem.mn := m.(name);
     ModSem.initial_mr := ε;
     ModSem.initial_st := tt↑;
@@ -310,7 +339,7 @@ Section MODSEM.
 
   Definition modsemL (mL : programL) (ge: SkEnv.t) : ModSemL.t := {|
     ModSemL.fnsems :=
-      List.map (fun '(mn, (fn, f)) => (fn, fun a => transl_all mn (cfun (eval_imp ge f) a))) mL.(prog_funsL);
+      List.map (fun '(mn, (fn, f)) => (fn, fun a => transl_all mn (cfun (eval_imp ge mL.(ext_funsL) f) a))) mL.(prog_funsL);
     ModSemL.initial_mrs :=
       List.map (fun name => (name, (ε, tt↑))) mL.(nameL);
   |}.
