imp/Imp2CsharpminorGenv.v
@@ -28,7 +28,8 @@ Section GENV.
         f mn fn impf
         (FOUND : find
                    ((fun '(k2, _) => f ?[ eq ] k2) <*>
-                    (fun '(mn, (fn, f)) => (fn, transl_all mn ∘ cfun (eval_imp (Sk.sort (defsL src)) f)))) (prog_funsL src) =
+                     (fun '(mn, (fn, f)) =>
+                      (fn, transl_all mn ∘ cfun (eval_imp (Sk.sort (defsL src)) (ext_funsL src) f)))) (prog_funsL src) =
                  Some (mn, (fn, impf)))
     :
       (fn = f) /\ (In (mn, (fn, impf)) (prog_funsL src)).
