imp/ImpProofs.v
@@ -29,7 +29,7 @@ Section PROOFS.
         ge le0 n
     :
       interp_imp ge (denote_expr (Lit n)) le0 =
-      interp_imp ge (assume (wf_val n);;; Ret n) le0.
+      interp_imp ge (assume (wf_val (Vint n));;; Ret (Vint n)) le0.
   Proof. reflexivity. Qed.
 
   Lemma denote_expr_Plus
@@ -56,90 +56,90 @@ Section PROOFS.
   (* stmt *)
 
   Lemma denote_stmt_Skip
-        ge le0
+        efs ge le0
     :
-      interp_imp ge (denote_stmt (Skip)) le0 =
+      interp_imp ge (denote_stmt efs (Skip)) le0 =
       interp_imp ge (tau;; Ret Vundef) le0.
   Proof. reflexivity. Qed.
 
   Lemma denote_stmt_Assign
-        ge le0 x e
+        efs ge le0 x e
     :
-      interp_imp ge (denote_stmt (Assign x e)) le0 =
+      interp_imp ge (denote_stmt efs (Assign x e)) le0 =
       interp_imp ge (v <- denote_expr e ;; trigger (SetVar x v) ;;; tau;; Ret Vundef) le0.
   Proof. reflexivity. Qed.
 
   Lemma denote_stmt_Seq
-        ge le0 a b
+        efs ge le0 a b
     :
-      interp_imp ge (denote_stmt (Seq a b)) le0 =
-      interp_imp ge (tau;; denote_stmt a ;;; denote_stmt b) le0.
+      interp_imp ge (denote_stmt efs (Seq a b)) le0 =
+      interp_imp ge (tau;; denote_stmt efs a ;;; denote_stmt efs b) le0.
   Proof. reflexivity. Qed.
 
   Lemma denote_stmt_If
-        ge le0 i t e
+        efs ge le0 i t e
     :
-      interp_imp ge (denote_stmt (If i t e)) le0 =
+      interp_imp ge (denote_stmt efs (If i t e)) le0 =
       interp_imp ge (v <- denote_expr i ;; `b: bool <- (is_true v)? ;; tau;;
-      if b then (denote_stmt t) else (denote_stmt e)) le0.
+      if b then (denote_stmt efs t) else (denote_stmt efs e)) le0.
   Proof. reflexivity. Qed.
 
   Lemma denote_stmt_AddrOf
-        ge le0 x X
+        efs ge le0 x X
     :
-      interp_imp ge (denote_stmt (AddrOf x X)) le0 =
+      interp_imp ge (denote_stmt efs (AddrOf x X)) le0 =
       interp_imp ge (v <- trigger (GetPtr X);; trigger (SetVar x v);;; tau;; Ret Vundef) le0.
   Proof. reflexivity. Qed.
 
   Lemma denote_stmt_Malloc
-        ge le0 x se
+        efs ge le0 x se
     :
-      interp_imp ge (denote_stmt (Malloc x se)) le0 =
+      interp_imp ge (denote_stmt efs (Malloc x se)) le0 =
       interp_imp ge (s <- denote_expr se;;
       v <- trigger (Call "alloc" ([s]↑));; v <- unwrapN(v↓);;
       trigger (SetVar x v);;; tau;; Ret Vundef) le0.
   Proof. reflexivity. Qed.
 
   Lemma denote_stmt_Free
-        ge le0 pe
+        efs ge le0 pe
     :
-      interp_imp ge (denote_stmt (Free pe)) le0 =
+      interp_imp ge (denote_stmt efs (Free pe)) le0 =
       interp_imp ge (p <- denote_expr pe;;
       trigger (Call "free" ([p]↑));;; tau;; Ret Vundef) le0.
   Proof. reflexivity. Qed.
 
   Lemma denote_stmt_Load
-        ge le0 x pe
+        efs ge le0 x pe
     :
-      interp_imp ge (denote_stmt (Load x pe)) le0 =
+      interp_imp ge (denote_stmt efs (Load x pe)) le0 =
       interp_imp ge (p <- denote_expr pe;;
       v <- trigger (Call "load" ([p]↑));; v <- unwrapN(v↓);;
       trigger (SetVar x v);;; tau;; Ret Vundef) le0.
   Proof. reflexivity. Qed.
 
   Lemma denote_stmt_Store
-        ge le0 pe ve
+        efs ge le0 pe ve
     :
-      interp_imp ge (denote_stmt (Store pe ve)) le0 =
+      interp_imp ge (denote_stmt efs (Store pe ve)) le0 =
       interp_imp ge (p <- denote_expr pe;; v <- denote_expr ve;;
       trigger (Call "store" ([p ; v]↑));;; tau;; Ret Vundef) le0.
   Proof. reflexivity. Qed.
 
   Lemma denote_stmt_Cmp
-        ge le0 x ae be
+        efs ge le0 x ae be
     :
-      interp_imp ge (denote_stmt (Cmp x ae be)) le0 =
+      interp_imp ge (denote_stmt efs (Cmp x ae be)) le0 =
       interp_imp ge ( a <- denote_expr ae;; b <- denote_expr be;;
       v <- trigger (Call "cmp" ([a ; b]↑));; v <- unwrapN (v↓);;
       trigger (SetVar x v);;; tau;; Ret Vundef) le0.
   Proof. reflexivity. Qed.
 
   Lemma denote_stmt_CallFun
-        ge le0 x f args
+        efs ge le0 x f args
     :
-      interp_imp ge (denote_stmt (CallFun x f args)) le0 =
+      interp_imp ge (denote_stmt efs (CallFun x f args)) le0 =
       interp_imp ge (
-      if (call_mem f)
+      if (call_ban f)
       then triggerUB
       else
         eval_args <- (denote_exprs args);;
@@ -148,12 +148,13 @@ Section PROOFS.
   Proof. reflexivity. Qed.
 
   Lemma denote_stmt_CallPtr
-        ge le0 x e args
+        efs ge le0 x e args
     :
-      interp_imp ge (denote_stmt (CallPtr x e args)) le0 =
+      interp_imp ge (denote_stmt efs (CallPtr x e args)) le0 =
       interp_imp ge (
+      assume (match e with | Var _ => True | _ => False end);;;
       p <- denote_expr e;; f <- trigger (GetName p);;
-      if (call_mem f)
+      if (call_ban f)
       then triggerUB
       else
         eval_args <- (denote_exprs args);;
@@ -162,10 +163,11 @@ Section PROOFS.
   Proof. reflexivity. Qed.
 
   Lemma denote_stmt_CallSys
-        ge le0 x f args
+        efs ge le0 x f args
     :
-      interp_imp ge (denote_stmt (CallSys x f args)) le0 =
+      interp_imp ge (denote_stmt efs (CallSys x f args)) le0 =
       interp_imp ge (
+      sig <- (alist_find f efs)? ;; assume (sig = List.length args);;;
       eval_args <- (denote_exprs args);;
       v <- trigger (Syscall f eval_args top1);;
       trigger (SetVar x v);;; tau;; Ret Vundef) le0.
@@ -360,7 +362,7 @@ Section PROOFS.
         ge le0 n
     :
       interp_imp ge (denote_expr (Lit n)) le0 =
-      assume (wf_val n);;; tau;; tau;; Ret (le0, n).
+      assume (wf_val (Vint n));;; tau;; tau;; Ret (le0, Vint n).
   Proof.
     rewrite denote_expr_Lit. rewrite interp_imp_bind. rewrite interp_imp_assume. grind. apply interp_imp_Ret.
   Qed.
@@ -417,9 +419,9 @@ Section PROOFS.
   Qed.
 
   Lemma interp_imp_Skip
-        ge le0
+        efs ge le0
     :
-      interp_imp ge (denote_stmt (Skip)) le0 =
+      interp_imp ge (denote_stmt efs (Skip)) le0 =
       tau;; Ret (le0, Vundef).
   Proof.
     rewrite denote_stmt_Skip. rewrite interp_imp_tau.
@@ -427,9 +429,9 @@ Section PROOFS.
   Qed.
 
   Lemma interp_imp_Assign
-        ge le0 x e
+        efs ge le0 x e
     :
-      interp_imp ge (denote_stmt (Assign x e)) le0 =
+      interp_imp ge (denote_stmt efs (Assign x e)) le0 =
       '(le1, v) <- interp_imp ge (denote_expr e) le0 ;;
       tau;; tau;; tau;; Ret (alist_add x v le1, Vundef).
   Proof.
@@ -441,26 +443,26 @@ Section PROOFS.
   Qed.
 
   Lemma interp_imp_Seq
-        ge le0 a b
+        efs ge le0 a b
     :
-      interp_imp ge (denote_stmt (Seq a b)) le0 =
+      interp_imp ge (denote_stmt efs (Seq a b)) le0 =
       tau;;
-      '(le1, _) <- interp_imp ge (denote_stmt a) le0 ;;
-      interp_imp ge (denote_stmt b) le1.
+      '(le1, _) <- interp_imp ge (denote_stmt efs a) le0 ;;
+      interp_imp ge (denote_stmt efs b) le1.
   Proof.
     rewrite denote_stmt_Seq. rewrite interp_imp_tau; grind.
     apply interp_imp_bind.
   Qed.
 
   Lemma interp_imp_If
-        ge le0 i t e
+        efs ge le0 i t e
     :
-      interp_imp ge (denote_stmt (If i t e)) le0 =
+      interp_imp ge (denote_stmt efs (If i t e)) le0 =
       '(le1, v) <- interp_imp ge (denote_expr i) le0 ;;
       `b: bool <- (is_true v)? ;; tau;;
        if b
-       then interp_imp ge (denote_stmt t) le1
-       else interp_imp ge (denote_stmt e) le1.
+       then interp_imp ge (denote_stmt efs t) le1
+       else interp_imp ge (denote_stmt efs e) le1.
   Proof.
     rewrite denote_stmt_If. rewrite interp_imp_bind. grind.
     destruct (is_true v); grind; des_ifs.
@@ -469,9 +471,9 @@ Section PROOFS.
   Qed.
 
   Lemma interp_imp_AddrOf
-        ge le0 x X
+        efs ge le0 x X
     :
-      interp_imp ge (denote_stmt (AddrOf x X)) le0 =
+      interp_imp ge (denote_stmt efs (AddrOf x X)) le0 =
       r <- (ge.(SkEnv.id2blk) X)? ;; tau;;
       tau;; tau;; tau;; Ret (alist_add x (Vptr r 0) le0, Vundef).
   Proof.
@@ -482,9 +484,9 @@ Section PROOFS.
   Qed.
 
   Lemma interp_imp_Malloc
-        ge le0 x se
+        efs ge le0 x se
     :
-      interp_imp ge (denote_stmt (Malloc x se)) le0 =
+      interp_imp ge (denote_stmt efs (Malloc x se)) le0 =
       '(le1, s) <- interp_imp ge (denote_expr se) le0;;
       v <- trigger (Call "alloc" ([s]↑));;
       tau;; tau;; v <- unwrapN (v↓);;
@@ -498,9 +500,9 @@ Section PROOFS.
   Qed.
 
   Lemma interp_imp_Free
-        ge le0 pe
+        efs ge le0 pe
     :
-      interp_imp ge (denote_stmt (Free pe)) le0 =
+      interp_imp ge (denote_stmt efs (Free pe)) le0 =
       '(le1, p) <- interp_imp ge (denote_expr pe) le0;;
       trigger (Call "free" ([p]↑));;; tau;; tau;; tau;; Ret (le1, Vundef).
   Proof.
@@ -510,9 +512,9 @@ Section PROOFS.
   Qed.
 
   Lemma interp_imp_Load
-        ge le0 x pe
+        efs ge le0 x pe
     :
-      interp_imp ge (denote_stmt (Load x pe)) le0 =
+      interp_imp ge (denote_stmt efs (Load x pe)) le0 =
       '(le1, p) <- interp_imp ge (denote_expr pe) le0;;
       v <- trigger (Call "load" ([p]↑));;
       tau;; tau;; v <- unwrapN (v↓);;
@@ -526,9 +528,9 @@ Section PROOFS.
   Qed.
 
   Lemma interp_imp_Store
-        ge le0 pe ve
+        efs ge le0 pe ve
     :
-      interp_imp ge (denote_stmt (Store pe ve)) le0 =
+      interp_imp ge (denote_stmt efs (Store pe ve)) le0 =
       '(le1, p) <- interp_imp ge (denote_expr pe) le0;;
       '(le2, v) <- interp_imp ge (denote_expr ve) le1;;
       trigger (Call "store" ([p ; v]↑));;; tau;; tau;; tau;; Ret (le2, Vundef).
@@ -540,9 +542,9 @@ Section PROOFS.
   Qed.
 
   Lemma interp_imp_Cmp
-        ge le0 x ae be
+        efs ge le0 x ae be
     :
-      interp_imp ge (denote_stmt (Cmp x ae be)) le0 =
+      interp_imp ge (denote_stmt efs (Cmp x ae be)) le0 =
       '(le1, a) <- interp_imp ge (denote_expr ae) le0;;
       '(le2, b) <- interp_imp ge (denote_expr be) le1;;
       v <- trigger (Call "cmp" ([a ; b]↑));;
@@ -578,10 +580,10 @@ Section PROOFS.
   Qed.
 
   Lemma interp_imp_CallFun
-        ge le0 x f args
+        efs ge le0 x f args
     :
-      interp_imp ge (denote_stmt (CallFun x f args)) le0 =
-      if (call_mem f)
+      interp_imp ge (denote_stmt efs (CallFun x f args)) le0 =
+      if (call_ban f)
       then triggerUB
       else
         '(le1, vals) <- interp_imp ge (denote_exprs args) le0;;
@@ -594,15 +596,16 @@ Section PROOFS.
   Qed.
 
   Lemma interp_imp_CallPtr
-        ge le0 x e args
+        efs ge le0 x e args
     :
-      interp_imp ge (denote_stmt (CallPtr x e args)) le0 =
+      interp_imp ge (denote_stmt efs (CallPtr x e args)) le0 =
+      assume (match e with | Var _ => True | _ => False end);;; tau;; tau;;
       '(le1, p) <- interp_imp ge (denote_expr e) le0;;
       match p with
       | Vptr n 0 =>
         match (SkEnv.blk2id ge n) with
         | Some f =>
-          if (call_mem f)
+          if (call_ban f)
           then tau;; triggerUB
           else
             tau;;
@@ -615,7 +618,9 @@ Section PROOFS.
       | _ => triggerUB
       end.
   Proof.
-    rewrite denote_stmt_CallPtr. rewrite interp_imp_bind. grind.
+    rewrite denote_stmt_CallPtr.
+    rewrite interp_imp_bind. rewrite interp_imp_assume. grind.
+    rewrite interp_imp_bind. grind.
     rewrite interp_imp_bind. rewrite interp_imp_GetName.
     des_ifs.
     1,5,6,7:(unfold triggerUB; grind).
@@ -644,47 +649,58 @@ Section PROOFS.
   Qed.
 
   Lemma interp_imp_CallSys
-        ge le0 x f args
+        efs ge le0 x f args
     :
-      interp_imp ge (denote_stmt (CallSys x f args)) le0 =
+      interp_imp ge (denote_stmt efs (CallSys x f args)) le0 =
+      sig <- (alist_find f efs)? ;; assume (sig = List.length args);;; tau;; tau;;
       '(le1, vals) <- interp_imp ge (denote_exprs args) le0;;
       v <- trigger (Syscall f vals top1);;
       tau;; tau;; tau;; tau;;
       tau;; Ret (alist_add x v le1, Vundef).
   Proof.
-    rewrite denote_stmt_CallSys. apply interp_imp_Syscall_args.
+    rewrite denote_stmt_CallSys.
+    rewrite interp_imp_bind. rewrite interp_imp_unwrapU. grind.
+    rewrite interp_imp_bind. rewrite interp_imp_assume. grind.
+    apply interp_imp_Syscall_args.
   Qed.
 
   (* eval_imp  *)
   Lemma unfold_eval_imp
-        ge fparams fvars fbody args
+        ge efs fparams fvars fbody args
     :
-      ` vret : val <- eval_imp ge (mk_function fparams fvars fbody) args ;; Ret (vret↑)
+      ` vret : val <- eval_imp ge efs (mk_function fparams fvars fbody) args ;; Ret (vret↑)
                =
                ` vret : val <-
-                        (match init_args fparams args [] with
-                         | Some iargs =>
-                           ` x_ : lenv * val <-
-                                  interp_imp ge (tau;; denote_stmt (fbody);;; ` retv : val <- denote_expr (Var "return");; Ret retv) (init_lenv (fvars) ++ iargs);;
-                                  (let (_, retv) := x_ in Ret retv)
-                         | None => triggerUB
-                         end) ;; Ret (vret↑).
+                        (
+                          let vars := fvars ++ ["return"; "_"] in
+                          let params := fparams in
+                          assume (NoDup (params ++ vars));;;
+                                 match init_args params args [] with
+                                 | Some iargs =>
+                                   ` x_ : lenv * val <-
+                                          interp_imp ge (tau;; denote_stmt efs fbody;;; ` retv : val <- denote_expr (Var "return");; Ret retv)
+                                                     (init_lenv vars ++ iargs);; (let (_, retv) := x_ in Ret retv)
+                                 | None => triggerUB
+                                 end);; Ret (vret↑).
   Proof.
     unfold eval_imp. ss.
   Qed.
 
   Lemma unfold_eval_imp_only
-        ge f args
+        ge efs f args
     :
-      eval_imp ge f args
+      eval_imp ge efs f args
       =
-      match init_args (fn_params f) args [] with
-      | Some iargs =>
-        ` x_ : lenv * val <-
-               interp_imp ge (tau;; denote_stmt (fn_body f);;; ` retv : val <- denote_expr (Var "return");; Ret retv) (init_lenv (fn_vars f) ++ iargs);;
-               (let (_, retv) := x_ in Ret retv)
-      | None => triggerUB
-      end.
+      let vars := fn_vars f ++ ["return"; "_"] in
+      let params := fn_params f in
+      assume (NoDup (params ++ vars));;;
+             match init_args params args [] with
+             | Some iargs =>
+               ` x_ : lenv * val <-
+                      interp_imp ge (tau;; denote_stmt efs (fn_body f);;; ` retv : val <- denote_expr (Var "return");; Ret retv)
+                                 (init_lenv vars ++ iargs);; (let (_, retv) := x_ in Ret retv)
+             | None => triggerUB
+             end.
   Proof. ss. Qed.
 
 End PROOFS.
@@ -705,7 +721,7 @@ Ltac imp_red :=
   cbn; try (rewrite interp_imp_bind);
   match goal with
   (** denote_stmt *)
-  | [ |- (gpaco6 (_sim_itree _) _ _ _ _ _ _ _ _ (_, ITree.bind' _ (interp_imp _ (denote_stmt (?stmt)) _))) ] =>
+  | [ |- (gpaco6 (_sim_itree _) _ _ _ _ _ _ _ _ (_, ITree.bind' _ (interp_imp _ (denote_stmt _ (?stmt)) _))) ] =>
     match stmt with
     | Skip => rewrite interp_imp_Skip
     | Assign _ _ => rewrite interp_imp_Assign
@@ -746,3 +762,4 @@ Ltac imp_red :=
   end.
 
 Ltac imp_steps := repeat (repeat imp_red; steps).
+Ltac solve_NoDup := repeat econs; ii; ss; des; ss.
